Progress, incl. a better `WellScopedEnv`, but still full of admits

examples/ghc/theories/CSE.v
@@ -1,5 +1,5 @@
 From Coq Require Import ssreflect ssrbool ssrfun.
-From mathcomp Require Import ssrnat.
+From mathcomp Require Import ssrnat eqtype.
 Set Bullet Behavior "Strict Subproofs".
 
 Generalizable All Variables.
@@ -51,6 +51,11 @@ Lemma cseExpr_Let env bind e :
                              in Let bind' (cseExpr env' e).
 Proof. done. Qed.
 Hint Rewrite cseExpr_Let : hs_simpl.
+
+Lemma cseExpr_Case env e bndr ty alts :
+  cseExpr env (Case e bndr ty alts) = cseCase env e bndr ty alts.
+Proof. done. Qed.
+Hint Rewrite cseExpr_Case : hs_simpl.
 
 Lemma cseBind_NonRec toplevel env b e :
   cseBind toplevel env (NonRec b e) =
@@ -117,12 +122,16 @@ Hint Rewrite (@stripTicksT_nil CoreBndr) : hs_simpl.
 
 (** * Well-scopedness for CSE *)
 
+Definition getCSEnvInScopeVars : CSEnv -> VarSet := getSubstInScopeVars ∘ cs_subst.
+Arguments getCSEnvInScopeVars !env /.
+
 (* vars = set of variables in scope AFTER `cs_subst` is applied *)
 Record WellScopedCSEnv (env : CSEnv) (vars : VarSet) : Prop :=
  IsWellScopedCSEnv
    { ws_subst   : WellScoped_Subst (cs_subst env) vars
-   ; ws_map     : TrieMap_All (WellScoped^~ vars) (cs_map env)
-   ; ws_rec_map : TrieMap_All (WellScoped^~ vars) (cs_rec_map env) }.
+   ; ws_map     : TrieMap_All (WellScoped^~ (getCSEnvInScopeVars env)) (cs_map env)
+   ; ws_rec_map : TrieMap_All (WellScoped^~ (getCSEnvInScopeVars env)) (cs_rec_map env) }.
+   (* `WellScoped^~ vars` or `WellScoped (getSubstInScopeVars (cs_subst env)`? *)
 
 Theorem WellScoped_Subst_subset subst vars :
   WellScoped_Subst subst vars ->
@@ -149,6 +158,83 @@ Qed.
 
 Ltac simpl_Key := rewrite /Key /TrieMap__CoreMap /TrieMap.TrieMap__CoreMap_Key.
 
+Lemma WellScoped_SetEq vars1 vars2 expr :
+  vars1 {=} vars2 ->
+  WellScoped expr vars1 <-> WellScoped expr vars2.
+Proof. by case=> ss12 ss21; split=> WS; eapply WellScoped_StrongSubset; eassumption. Qed.
+
+Lemma SubstExtends_WellScoped_iff sub v sub' v' expr :
+  SubstExtends sub (v :: nil) sub' (v' :: nil) ->
+  WellScoped expr (getSubstInScopeVars sub') <-> WellScoped expr (extendVarSet (getSubstInScopeVars sub) v').
+Proof.
+  case: sub => [in_scope id_env tm cm]; case: sub' => [in_scope' id_env' tm' cm'].
+  rewrite /SubstExtends /=; hs_simpl; move=> [_ [_ [_ [FL [inScopeVars_eq [minusDom_subst VEE]]]]]].
+  by rewrite (WellScoped_SetEq (_ in_scope')); last eassumption.
+Qed.
+
+Lemma SubstExtends_WellScoped_iff_eta1 in_scope id_env tm cm v sub' v' expr :
+  SubstExtends (Mk_Subst in_scope id_env tm cm) (v :: nil) sub' (v' :: nil) ->
+  WellScoped expr (getSubstInScopeVars sub') <-> WellScoped expr (extendVarSet (getInScopeVars in_scope) v').
+Proof. apply SubstExtends_WellScoped_iff. Qed.
+
+Lemma SubstExtends_WellScoped_preserved sub v sub' v' expr :
+  SubstExtends sub (v :: nil) sub' (v' :: nil) ->
+  WellScoped expr (getSubstInScopeVars sub) -> WellScoped expr (getSubstInScopeVars sub').
+Proof.
+  move=> SE.
+  rewrite (SubstExtends_WellScoped_iff _ _ sub'); last eassumption.
+  move=> /WellScoped_StrongSubset; apply.
+  apply StrongSubset_extend_fresh.
+  by move: sub sub' SE => [? ? ? ?] [? ? ? ?] [_ [_ [_ [/freshList_cons[? ?] _]]]].
+Qed.  
+
+Ltac do_Expand_substBndr def_subst'_v' subst' v' def_subst' in_scope' id_env' tm' cm' :=
+  match goal with
+  | |- context[substBndr ?subst ?v] => case def_subst'_v': (substBndr subst v) => [subst' v']
+  end;
+  let H := fresh in
+  case H: subst' => [in_scope' id_env' tm' cm']; rewrite -H; rename H into def_subst'.
+  (* For some reason, if `def_subst'` is passed in as an `ident`, it can't be
+     used in `rewrite`, so we go through an intermediate `H` *)
+
+Tactic Notation "Expand_substBndr" "=>"
+                ident(def_subst'_v') "[" ident(subst') ident(v') "]"
+                ident(def_subst')    "[" ident(in_scope') ident(id_env') ident(tm') ident(cm') "]" :=
+  do_Expand_substBndr def_subst'_v' subst' v' def_subst' in_scope' id_env' tm' cm'.
+
+Ltac GoodLocalVar_WellScoped_substBndr :=
+  match goal with
+  | SB  : substBndr ?subst ?v = (?subst',?bndr')
+  , GLV : GoodLocalVar ?v
+  , WSS : WellScoped_Subst ?subst ?vs
+    |- _ => move: (GoodLocalVar_substBndr     v bndr' subst subst' GLV SB)
+                  (WellScoped_Subst_substBndr subst subst' bndr'  v vs SB GLV WSS)
+  end. 
+
+Inductive Expr_Var_View {b} : Expr b -> Type :=
+| EVV_IsVar  v : Expr_Var_View (Mk_Var v)
+| EVV_NotVar e : ~ (exists v, e = Mk_Var v) -> Expr_Var_View e.
+
+Definition case_if_Var {b} (e : Expr b) : Expr_Var_View e :=
+  match e with
+  | Mk_Var v => EVV_IsVar  v
+  | e'       => EVV_NotVar e' ltac:(by subst e'; move=> [v ?])
+  end.
+
+Ltac lapply_all H :=
+  match type of H with
+  | (_ -> _) => lapply H; try clear H; first (let G := fresh in move=> G; lapply_all G)
+  | _        => move: H
+  end.
+
+Lemma GoodLocalVar_zapIdOccInfo v :
+  GoodLocalVar v ->
+  GoodLocalVar (zapIdOccInfo v).
+Proof.
+  case: v => [varName realUnique varType idScope id_details id_info].
+  by move=> []; repeat move=> [] ?; repeat split.
+Qed.
+
 Definition WS_cseExpr vars env e :
   WellScopedCSEnv env             vars ->
   WellScoped      e               vars ->
@@ -161,7 +247,7 @@ Proof.
     | e ty IH
     | co | ty ]
     vars
-    [[in_scope id_env tm cm] cs_map cs_rec_map]
+    [cs_sub cs_map cs_rec_map]
     //; hs_simpl;
     move=> WSenv; move: (WSenv) => [WSsubst WSmap WSrec];
     rewrite /cs_subst in WSsubst; rewrite /CSE.cs_map in WSmap; rewrite /CSE.cs_rec_map in WSrec.
@@ -172,61 +258,188 @@ Proof.
   - move=> /= [WSe1 WSe2]; split; first by apply (IH1 vars).
     rewrite tryForCSE_simpl /=.
     case LOOKUP: (lookupCoreMap _ _) => [e|]; last by apply (IH2 vars).
-    eapply TrieMap_All_lookup_Some in LOOKUP; last eassumption; simpl in LOOKUP.
-    eapply WellScoped_StrongSubset; first by apply LOOKUP.
-    by apply WellScoped_Subst_subset in WSsubst.
+    by eapply TrieMap_All_lookup_Some in LOOKUP => //.
   
   - rewrite /= /addBinder /= => -[GLV WSe].
-    case SB: (substBndr _ _) => [sub' v'] /=.
-    move: (WellScoped_Subst_substBndr _ _ _ _ _ SB GLV WSsubst) => [SE WSsubst'].
-    move: (GoodLocalVar_substBndr _ _ _ _ GLV SB) => GLV'.
+    case SB: (substBndr _ _) => [sub' v'].
+    GoodLocalVar_WellScoped_substBndr => GLV' [SE WSsubst'].
     split=> //.
     specialize (IH (extendVarSet vars v) (CS sub' cs_map cs_rec_map)).
-    case def_sub': sub' IH SB SE WSsubst' => [in_scope' id_env' tm' cm'];
-      rewrite -!def_sub' => IH SB SE WSsubst'.
-    move: (SE); rewrite {1}def_sub' /SubstExtends /=; hs_simpl.
-    move=> [_ [_ [_ [FL [inScopeVars_eq [minusDom_subset VEE]]]]]].
-    move: FL => /freshList_cons [fresh_v' _].
-    lapply IH; first move=> {IH} IH.
-    + move: IH; rewrite /cs_subst => /(_ WSe) IH.
-      apply WellScoped_StrongSubset with (vs1 := getSubstInScopeVars sub') => //.
-      by rewrite def_sub'; case: inScopeVars_eq.
+    lapply_all IH => //.
+    + by rewrite -SubstExtends_WellScoped_iff; last eassumption; apply.
     + constructor=> //; rewrite /cs_subst //=.
-      * eapply TrieMap_All_impl_lookup; last eassumption.
-        simpl_Key.
-        move=> k v''.
-
-        clear
-        
-        
-        move=> /= v'' /=.
-        apply WellScoped_extendVarSet_fresh
+      all: by eapply TrieMap_All_impl_lookup => // *; eauto using SubstExtends_WellScoped_preserved.
 
   - rewrite (lock cse_bind) /= -(lock cse_bind) => -[[GLV WS_rhs] WS_ext].
-    rewrite /addBinder /substBndr isn'tTyVar isn'tCoVar.
-    case def_sub'_v': (substIdBndr _ _ _ _) => [sub' v'].
-    have GLV': GoodLocalVar v' by eapply GoodLocalVar_substIdBndr; eassumption.
-    move: (WellScoped_Subst_substIdBndr _ _ _ _ _ _ _ def_sub'_v' GLV WSsubst)
-      => [subst_ext WSsubst'].
+    rewrite /addBinder.
+    case def_sub'_v': (substBndr _ _) => [sub' v'].
+    GoodLocalVar_WellScoped_substBndr => GLV' [SE WSsubst'].
     
     (* cse_bind *)
     simpl.
+    rewrite tryForCSE_simpl.
     case def_env'_out_id': (addBinding _ _ _ _) => [env' out_id'].
     case join_v: (isJoinId_maybe v) => [arity|].
     + admit.
-    + rewrite tryForCSE_simpl /=.
+    + move: def_env'_out_id' => /=.
       case LOOKUP: (lookupCoreMap _ _) => [e|]; hs_simpl.
-      * admit.
-      * split; first split.
-        -- admit.
-        -- admit. (* IHbind *)
-        -- (* ? *)
-           suff <-: getSubstInScopeVars (cs_subst env') = extendVarSet (getInScopeVars in_scope) out_id'. {
-             eapply IHbody; last eassumption; hs_simpl.
-             constructor => //.
+      * rewrite /addBinding; hs_simpl => /=.
+        case testCSE: (noCSE v).
+        -- move=> [? ?]; subst env' out_id'.
+           split; first split=> //.
+           ++ by eapply TrieMap_All_lookup_Some in LOOKUP; last eassumption.
+           ++ lapply_all (IHbody (extendVarSet vars v) (CS sub' cs_map cs_rec_map)) => //=.
+              ** by rewrite -SubstExtends_WellScoped_iff; last eassumption.
+              ** constructor => //=.
+                 all: eapply TrieMap_All_impl_lookup; last eassumption;
+                      eauto using SubstExtends_WellScoped_preserved.
+        -- destruct (case_if_Var e) as [ev|e e_nonvar] => //=; hs_simpl.
+           ++ move=> [<-{env'} <-{out_id'}].
+              split; first split=> //.
+              ** by eapply TrieMap_All_lookup_Some in LOOKUP; last eassumption.
+              ** move: (WSsubst'); rewrite (lock WellScoped_Subst); case: sub' def_sub'_v' SE WSsubst' LOOKUP
+                   => [in_scope' id_env' tm' cm'] //= def_sub'_v' SE [WSsubst'_SS WSsubst'_lookup] LOOKUP;
+                   hs_simpl; rewrite -(lock WellScoped_Subst) => WSsubst'.
+                 rewrite -SubstExtends_WellScoped_iff; last eassumption.
+                 eapply IHbody; last eassumption; hs_simpl.
+                 constructor.
+                 all: try by eapply TrieMap_All_impl_lookup; last eassumption;
+                             move=> ? ? ? H; eapply SubstExtends_WellScoped_preserved in H; last eassumption.
+                 rewrite /cs_subst.
+                 split.
+                 --- etransitivity; first by apply StrongSubset_minusDom_extend_extend.
+                     etransitivity; last by apply WSsubst'_SS.
+                     
+                     (*destruct cs_sub as [in_scope id_env tm cm] eqn:def_cs_sub.
+                     move: (SE)
+                       => [/= _ [_ [_ [/freshList_cons [fresh_v _] [inScopeVars_eq [minusDom_subst VEE]]]]]].
+                     move: minusDom_subst.
+                     replace (getInScopeVars in_scope')
+                       with  (extendVarSetList (getInScopeVars in_scope) (v' :: nil))
+                       by admit.
+                     hs_simpl.
+                     
+                     etransitivity; first by apply StrongSubset_minusDom_extend_extend.
+                     etransitivity; last by apply WSsubst'_SS.
+                     
+                     destruct cs_sub as [in_scope id_env tm cm] eqn:def_cs_sub.
+                     move: (SE)
+                       => [/= _ [_ [_ [/freshList_cons [fresh_v _] [inScopeVars_eq [minusDom_subst VEE]]]]]].
+                     replace (getInScopeVars in_scope')
+                       with  (extendVarSetList (getInScopeVars in_scope) (v' :: nil))
+                       by admit.
+                     hs_simpl.
+                     etransitivity; first by apply StrongSubset_minusDom_extend_extend.
+                     etransitivity; last by apply WSsubst'_SS.
+                     setoid_rewrite inScopeVars_eq.
+                     
+                     etransitivity; first by apply StrongSubset_minusDom_extend_extend.
+                     etransitivity; last by apply WSsubst'_SS.
+                     
+
+                     apply StrongSubset_extendVarSet_fresh.
+                     move: WS_ext; hs_simpl.
+                     rewrite /WellScoped*)
+                   admit.
+                     
+                 --- move=> var; specialize (WSsubst'_lookup var).
+                     case CMP: (v == var); [ rewrite lookupVarEnv_extendVarEnv_eq //
+                                           | rewrite lookupVarEnv_extendVarEnv_neq // CMP // ].
+                     eapply TrieMap_All_lookup_Some in LOOKUP; last eassumption.
+                     by eapply SubstExtends_WellScoped_preserved in LOOKUP; last eassumption.
+                 
+           ++ replace (match e with Mk_Var _ => _ | _ => false end) with false by
+                by case: e {LOOKUP} e_nonvar => //= ev []; exists ev.
+              move=> [<-{env'} <-{out_id'}].
+              split; first split.
+              ** by destruct v'.
+              ** by eapply TrieMap_All_lookup_Some in LOOKUP; last eassumption.
+              ** (*suff: forall expr vars var, WellScoped expr (extendVarSet vars var) -> WellScoped expr (extendVarSet vars (zapIdUsageInfo var)).
+                 {
+                   apply.
+                   eapply SubstExtends_WellScoped_iff; first eassumption.
+                   eapply IHbody; last eassumption.
+                   hs_simpl.
+                   constructor=> //.
+                   eapply TrieMap_All_impl_lookup.
+                   2: { simpl.
+                        apply TrieMap_All_insert; last eassumption.
+                        - admit.
+                        - rewrite /= /varToCoreExpr; hs_simpl=> /=.
+                          suff: (forall subst subst' v v',
+                                    GoodLocalVar v ->
+                                    substBndr subst v = (subst',v') ->
+                                    WellScopedVar v' (getSubstInScopeVars subst)).
+                          {
+                            by apply; last eassumption.
+                          }
+                            
+                          {
+                            clear=> -[in_scope id_env tm cm] subst' v v' GLV.
+                            rewrite /= /substBndr; hs_simpl => /=; hs_simpl=> /=.
+                            case CMP: (_ == _) => /=.
+                            - move=> [_ <-{v'}].
+                              rewrite Axioms.uniqAway_eq_same //.
+                              admit.
+                            - move=> [_ <-{v'}].
+                              red.
+                              case ILV: (isLocalVar _).
+                              + case LOOKUP: (lookupVarSet _ _) => [v'|].
+                                * split; last by apply GoodLocalVar_uniqAway.
+                                  destruct v; simpl in *.
+                                  rewrite /uniqAway.
+                                  case EISS: (elemInScopeSet _ _).
+                                  -- rewrite /uniqAway'.
+                                     rewrite /setVarUnique.
+                                     rewrite /Name.setNameUnique.
+                                     rewrite /Core.varName.
+                              + by apply GoodLocalVar_uniqAway.
+                            
+
+                          apply SubstExtends_WellScoped_iff.
+                          
+                          simpl in SE.
+                          case: SE => //= [_ [_ [_ X]]].
+                          destruct cs_sub as [in_scope id_env tm cm], sub' as [in_scope' id_env' tm' cm'].
+                          simpl.
+                          apply 
+                          
+                 all: try by eapply TrieMap_All_impl_lookup; last eassumption
+                             move=> ? ? ? H; SubstExtends_WellScoped_preserved in H; last eassumption.
+                 }
+              *)
+                admit.
+      * rewrite /addBinding; hs_simpl=> /=.
+        case testCSE: (noCSE v).
+        -- move => [<-{env'} <-{out_id'}].
+           split; first split=> //.
+           ++ (* suff: WellScoped (cseExpr (CS sub' cs_map cs_rec_map) rhs) (getSubstInScopeVars sub') ->
+                    WellScoped (cseExpr (CS sub' cs_map cs_rec_map) rhs) (getSubstInScopeVars cs_sub).
+              {
+                apply.
+                eapply IHbind; last eassumption.
+                constructor=> //=.
+                all: try (eapply TrieMap_All_impl_lookup; last eassumption; simpl).
+                all: try by move=> *; eapply SubstExtends_WellScoped_preserved; first eassumption.
+                
+              }
+              *)
              admit.
-           }
-           admit.
+           ++ eapply SubstExtends_WellScoped_iff; first eassumption.
+              eapply IHbody; last eassumption.
+              hs_simpl; constructor=> //.
+              all: eapply TrieMap_All_impl_lookup; last eassumption.
+              all: move=> ? ? LOOKUP' ?; eapply SubstExtends_WellScoped_preserved; first eassumption.
+              all: by eapply TrieMap_All_lookup_Some in LOOKUP'; last eassumption.
+        -- move def_rhs': (cseExpr (CS sub' cs_map cs_rec_map) rhs) => rhs'.
+           destruct (case_if_Var rhs') as [rhs'_v|rhs' rhs'_nonvar] => //=; hs_simpl;
+             last replace (match rhs' with Mk_Var _ => _ | _ => false end) with false by
+                    (by case: rhs' {def_rhs'} rhs'_nonvar => //= rhs'_v []; exists rhs'_v);
+             move=> [<-{env'} <-{out_id'}].
+           ++ split; first split=> //.
+              ** admit.
+              ** admit.
+           ++ admit.
 
   - rewrite (lock cseBind) /= -(lock cseBind).
     case: pairs IHbind => [|[in_id rhs] [|[in_id' rhs'] pairs]] IHbind [[GLVs [Uniq WS_pairs]] WS_body] /=.
@@ -235,18 +448,20 @@ Proof.
     + case checkCSE: (noCSE in_id).
       * simpl; hs_simpl.
         repeat split; try constructor=> //=.
-        -- apply GoodLocalVar_uniqAway.
-           by inversion_clear GLVs.
-        -- admit. (* IHbind *)
-        -- admit. (* IHbody *)
-      * case LOOKUP: (lookupCoreMap _ _) => [e|]; hs_simpl.
-        -- admit.
-        -- admit.
+        -- (*apply GoodLocalVar_uniqAway.
+           by inversion_clear GLVs.*)
+          admit.
+      * admit. (*case LOOKUP: (lookupCoreMap _ _) => [e|]; hs_simpl.*)
     + admit.
 
-  - admit.
+  - rewrite /= /cseCase => -[WS_scrut [GLV_bndr All_alts]].
+    rewrite /addBinder /=.
+    case def_sub'_v': (substBndr _ _) => [sub' v'].
+    move: (GoodLocalVar_zapIdOccInfo bndr GLV_bndr) => GLV_zap.
+    GoodLocalVar_WellScoped_substBndr => GLV' [SE WSsubst'].
+    admit.
 
   - simpl; hs_simpl.
     case def_e': (lookupCoreMap _ _) => [e'|]; hs_simpl; last by apply IH.
-    admit.
+    by eapply TrieMap_All_lookup_Some in def_e'; last eassumption; simpl in def_e'.
 Admitted.
